src/spec/TLS13.Wire.Spec.fsti
@@ -584,6 +584,12 @@ val lemma_serialize_tls_message_close_notify:
   Lemma (serialize_tls_message (M.TlsAlert T.Close_notify) ==
     (T.Alert, B.of_list [2uy; 0uy]))
 
+val lemma_parse_serialize_tls_message_close_notify:
+  unit ->
+  Lemma
+    (let (ct, frag) = serialize_tls_message (M.TlsAlert T.Close_notify) in
+     parse_tls_message ct frag == Some (M.TlsAlert T.Close_notify))
+
 val lemma_serialize_tls_message_change_cipher_spec:
   unit ->
   Lemma (serialize_tls_message M.TlsChangeCipherSpec ==
